code/experimental/rsa/Hacl.RSAPSS.fst
@@ -12,42 +12,42 @@ open Hacl.Impl.MGF
 module Buffer = Spec.Lib.IntBuf
 
 val rsa_pss_sign:
-    #sLen:size_nat -> #msgLen:size_nat ->
-    pow2_i:size_t -> iLen:size_t ->
-    modBits:size_t{0 < v modBits /\ v modBits + 3 < max_size_t} ->
+    #sLen:size_nat -> #msgLen:size_nat -> #nLen:size_nat ->
+    pow2_i:size_t{9 * (1 + nLen) + 4 * v pow2_i < max_size_t /\ (1 + nLen) < v pow2_i} ->
+    iLen:size_t{v iLen < v pow2_i / 2 /\ v iLen + (1 + nLen) = v pow2_i} ->
+    modBits:size_t{0 < v modBits /\ nLen = v (bits_to_bn modBits)} ->
     eBits:size_t{0 < v eBits /\ v eBits <= v modBits} ->
     dBits:size_t{0 < v dBits /\ v dBits <= v modBits} ->
-    pLen:size_t -> qLen:size_t{v (bits_to_bn modBits) + v (bits_to_bn eBits) + v (bits_to_bn dBits) + v pLen + v qLen < max_size_t} ->
-    skey:lbignum (v (bits_to_bn modBits) + v (bits_to_bn eBits) + v (bits_to_bn dBits) + v pLen + v qLen) ->
+    pLen:size_t -> qLen:size_t{nLen + v (bits_to_bn eBits) + v (bits_to_bn dBits) + v pLen + v qLen < max_size_t} ->
+    skey:lbignum (nLen + v (bits_to_bn eBits) + v (bits_to_bn dBits) + v pLen + v qLen) ->
     rBlind:uint64 ->
-    ssLen:size_t{v ssLen == sLen /\ sLen + v hLen + 8 < max_size_t /\ v (blocks modBits (size 8)) - sLen - v hLen - 3 >= 0 } ->
-    salt:lbytes sLen ->
+    ssLen:size_t{v ssLen == sLen /\ sLen + v hLen + 8 < max_size_t /\ v (blocks modBits (size 8)) - sLen - v hLen - 3 >= 0} -> salt:lbytes sLen ->
     mmsgLen:size_t{v mmsgLen == msgLen /\ msgLen < pow2 61} -> msg:lbytes msgLen ->
     sgnt:lbytes (v (blocks modBits (size 8))) -> Stack unit
     (requires (fun h -> live h salt /\ live h msg /\ live h sgnt /\ live h skey /\
 	              disjoint msg salt /\ disjoint msg sgnt /\ disjoint sgnt salt))
     (ensures (fun h0 _ h1 -> preserves_live h0 h1 /\ modifies1 sgnt h0 h1))
 
-let rsa_pss_sign #sLen #msgLen pow2_i iLen modBits eBits dBits pLen qLen skey rBlind ssLen salt mmsgLen msg sgnt =
-    push_frame();
-    Hacl.Impl.RSA.rsa_sign #sLen #msgLen pow2_i iLen modBits eBits dBits pLen qLen skey rBlind ssLen salt mmsgLen msg sgnt;
-    pop_frame()
+let rsa_pss_sign #sLen #msgLen #nLen pow2_i iLen modBits eBits dBits pLen qLen skey rBlind ssLen salt mmsgLen msg sgnt =
+    //push_frame();
+    Hacl.Impl.RSA.rsa_sign #sLen #msgLen #nLen pow2_i iLen modBits eBits dBits pLen qLen skey rBlind ssLen salt mmsgLen msg sgnt
+    //pop_frame()
 
 val rsa_pss_verify:
-    #sLen:size_nat -> #msgLen:size_nat ->
-    pow2_i:size_t -> iLen:size_t ->
-    modBits:size_t{0 < v modBits /\ v modBits + 3 < max_size_t} ->
-    eBits:size_t{0 < v eBits /\ v eBits <= v modBits /\
-		 v (bits_to_bn modBits) + v (bits_to_bn eBits) < max_size_t} ->
-    pkey:lbignum (v (bits_to_bn modBits) + v (bits_to_bn eBits)) ->
-    ssLen:size_t{v ssLen == sLen /\ sLen + v hLen + 8 < max_size_t} ->
+    #sLen:size_nat -> #msgLen:size_nat -> #nLen:size_nat ->
+    pow2_i:size_t{9 * (1 + nLen) + 4 * v pow2_i < max_size_t /\ (1 + nLen) < v pow2_i} ->
+    iLen:size_t{v iLen < v pow2_i / 2 /\ v iLen + (1 + nLen) = v pow2_i} ->
+    modBits:size_t{0 < v modBits /\ nLen = v (bits_to_bn modBits)} ->
+    eBits:size_t{0 < v eBits /\ v eBits <= v modBits /\ nLen + v (bits_to_bn eBits) < max_size_t} ->
+    pkey:lbignum (nLen + v (bits_to_bn eBits)) ->
+    ssLen:size_t{v ssLen == sLen /\ sLen + v hLen + 8 < max_size_t /\ v (blocks modBits (size 8)) - sLen - v hLen - 3 >= 0} ->
     sgnt:lbytes (v (blocks modBits (size 8))) ->
     mmsgLen:size_t{v mmsgLen == msgLen /\ msgLen < pow2 61} -> msg:lbytes msgLen -> Stack bool
     (requires (fun h -> live h msg /\ live h sgnt /\ live h pkey /\ disjoint msg sgnt))
     (ensures (fun h0 _ h1 -> preserves_live h0 h1 /\ modifies0 h0 h1))
 
-let rsa_pss_verify #sLen #msgLen pow2_i iLen modBits eBits pkey ssLen sgnt mmsgLen msg =
-    push_frame();
+let rsa_pss_verify #sLen #msgLen #nLen pow2_i iLen modBits eBits pkey ssLen sgnt mmsgLen msg =
+    //push_frame();
     let res = Hacl.Impl.RSA.rsa_verify #sLen #msgLen pow2_i iLen modBits eBits pkey ssLen sgnt mmsgLen msg in
-    pop_frame();
+    //pop_frame();
     res
